iris/IregDirBit.v
@@ -104,7 +104,7 @@ Section IregDirBit.
     iDestruct (ireg_slots_acc_upd γi (ireg_bi inum) ds (islot inum) Hsl Hlen16
                 with "Hsls") as "[Hslot Hslback]".
     iEval (rewrite Hkey) in "Hslot".
-    iDestruct "Hslot" as "[(%wl & %wdu & %wdt & %gl & %rl & %cl & %pl & Hla & %Hlok & %Hrt & %Hdir & %Hwl0 & %Hpar & #Hdisj) [Hep Harm]]".
+    iDestruct "Hslot" as "[(%wl & %wdu & %wdt & %gl & %rl & %cl & %pl & %fz & %cn & Hla & %Hlok & %Hrt & %Hdir & %Hwl0 & %Hpar & #Hdisj & Hcnt & %Hclm & %Hfrz & Hfdisj & Harm) Hep]".
     iDestruct (link_wd_ge with "Hla Hfrag") as %Hw1.
     rewrite /dinode_at.
     iDestruct (ghost_map_lookup with "Ha Hdn") as %Hm.
@@ -119,17 +119,17 @@ Section IregDirBit.
                ltac:(lia)). }
     assert (Hins : <[islot inum := ds !!! islot inum]> ds = ds).
     { apply list_insert_id, list_lookup_lookup_total_lt. lia. }
-    iMod ("Hclose" with "[Ha Hreg Hfsb Harm Hla Hep Hslback Hback]") as "_".
+    iMod ("Hclose" with "[Ha Hreg Hfsb Harm Hla Hep Hslback Hback Hcnt Hfdisj]") as "_".
     { iNext. iExists m. iFrame "Ha Hreg".
-      iApply ("Hback" $! m with "[%] [Hfsb Harm Hla Hep Hslback]"); [done |].
+      iApply ("Hback" $! m with "[%] [Hfsb Harm Hla Hep Hslback Hcnt Hfdisj]"); [done |].
       iExists ds. iSplitR; [done |]. iSplitR; [done |].
       iSplitL "Hfsb"; [iExact "Hfsb" |].
       iEval (rewrite -Hins).
-      iApply ("Hslback" $! (ds !!! islot inum) with "[Harm Hla Hep]").
+      iApply ("Hslback" $! (ds !!! islot inum) with "[Harm Hla Hep Hcnt Hfdisj]").
       rewrite Hkey.
       iApply (ireg_slot_intro γi (bv_unsigned inum) (ds !!! islot inum)
-                wl wdu wdt gl cl rl pl Hlok Hrt Hdir Hwl0 Hpar
-                with "Hla Hep Hdisj"). iExact "Harm". }
+                wl wdu wdt gl cl rl pl fz cn Hlok Hrt Hdir Hwl0 Hpar Hclm Hfrz
+                with "Hla Hep Hdisj Hcnt Hfdisj"). iExact "Harm". }
     iModIntro. iFrame "Hdn Hfrag". iPureIntro. exact Hty.
   Qed.
 
@@ -165,7 +165,7 @@ Section IregDirBit.
     iDestruct (ireg_slots_acc_upd γi (ireg_bi inum) ds (islot inum) Hsl Hlen16
                 with "Hsls") as "[Hslot Hslback]".
     iEval (rewrite Hkey) in "Hslot".
-    iDestruct "Hslot" as "[(%wl & %wdu & %wdt & %gl & %rl & %cl & %pl & Hla & %Hlok & %Hrt & %Hdir & %Hwl0 & %Hpar & #Hdisj) [Hep Harm]]".
+    iDestruct "Hslot" as "[(%wl & %wdu & %wdt & %gl & %rl & %cl & %pl & %fz & %cn & Hla & %Hlok & %Hrt & %Hdir & %Hwl0 & %Hpar & #Hdisj & Hcnt & %Hclm & %Hfrz & Hfdisj & Harm) Hep]".
     iDestruct (link_wdt_ge with "Hla Hfrag") as %[Hw1 _].
     rewrite /dinode_at.
     iDestruct (ghost_map_lookup with "Ha Hdn") as %Hm.
@@ -180,17 +180,17 @@ Section IregDirBit.
                ltac:(lia)). }
     assert (Hins : <[islot inum := ds !!! islot inum]> ds = ds).
     { apply list_insert_id, list_lookup_lookup_total_lt. lia. }
-    iMod ("Hclose" with "[Ha Hreg Hfsb Harm Hla Hep Hslback Hback]") as "_".
+    iMod ("Hclose" with "[Ha Hreg Hfsb Harm Hla Hep Hslback Hback Hcnt Hfdisj]") as "_".
     { iNext. iExists m. iFrame "Ha Hreg".
-      iApply ("Hback" $! m with "[%] [Hfsb Harm Hla Hep Hslback]"); [done |].
+      iApply ("Hback" $! m with "[%] [Hfsb Harm Hla Hep Hslback Hcnt Hfdisj]"); [done |].
       iExists ds. iSplitR; [done |]. iSplitR; [done |].
       iSplitL "Hfsb"; [iExact "Hfsb" |].
       iEval (rewrite -Hins).
-      iApply ("Hslback" $! (ds !!! islot inum) with "[Harm Hla Hep]").
+      iApply ("Hslback" $! (ds !!! islot inum) with "[Harm Hla Hep Hcnt Hfdisj]").
       rewrite Hkey.
       iApply (ireg_slot_intro γi (bv_unsigned inum) (ds !!! islot inum)
-                wl wdu wdt gl cl rl pl Hlok Hrt Hdir Hwl0 Hpar
-                with "Hla Hep Hdisj"). iExact "Harm". }
+                wl wdu wdt gl cl rl pl fz cn Hlok Hrt Hdir Hwl0 Hpar Hclm Hfrz
+                with "Hla Hep Hdisj Hcnt Hfdisj"). iExact "Harm". }
     iModIntro. iFrame "Hdn Hfrag". iPureIntro. exact Hty.
   Qed.
 
@@ -229,7 +229,7 @@ Section IregDirBit.
     iDestruct (ireg_slots_acc_upd γi (ireg_bi inum) ds (islot inum) Hsl Hlen16
                 with "Hsls") as "[Hslot Hslback]".
     iEval (rewrite Hkey) in "Hslot".
-    iDestruct "Hslot" as "[(%wl & %wdu & %wdt & %gl & %rl & %cl & %pl & Hla & %Hlok & %Hrt & %Hdir & %Hwl0 & %Hpar & #Hdisj) [Hep Harm]]".
+    iDestruct "Hslot" as "[(%wl & %wdu & %wdt & %gl & %rl & %cl & %pl & %fz & %cn & Hla & %Hlok & %Hrt & %Hdir & %Hwl0 & %Hpar & #Hdisj & Hcnt & %Hclm & %Hfrz & Hfdisj & Harm) Hep]".
     iDestruct (link_w_ge with "Hla Hfrag") as %Hw1.
     rewrite /dinode_at.
     iDestruct (ghost_map_lookup with "Ha Hdn") as %Hm.
@@ -245,17 +245,17 @@ Section IregDirBit.
       pose proof (Hwl0 Hc'). lia. }
     assert (Hins : <[islot inum := ds !!! islot inum]> ds = ds).
     { apply list_insert_id, list_lookup_lookup_total_lt. lia. }
-    iMod ("Hclose" with "[Ha Hreg Hfsb Harm Hla Hep Hslback Hback]") as "_".
+    iMod ("Hclose" with "[Ha Hreg Hfsb Harm Hla Hep Hslback Hback Hcnt Hfdisj]") as "_".
     { iNext. iExists m. iFrame "Ha Hreg".
-      iApply ("Hback" $! m with "[%] [Hfsb Harm Hla Hep Hslback]"); [done |].
+      iApply ("Hback" $! m with "[%] [Hfsb Harm Hla Hep Hslback Hcnt Hfdisj]"); [done |].
       iExists ds. iSplitR; [done |]. iSplitR; [done |].
       iSplitL "Hfsb"; [iExact "Hfsb" |].
       iEval (rewrite -Hins).
-      iApply ("Hslback" $! (ds !!! islot inum) with "[Harm Hla Hep]").
+      iApply ("Hslback" $! (ds !!! islot inum) with "[Harm Hla Hep Hcnt Hfdisj]").
       rewrite Hkey.
       iApply (ireg_slot_intro γi (bv_unsigned inum) (ds !!! islot inum)
-                wl wdu wdt gl cl rl pl Hlok Hrt Hdir Hwl0 Hpar
-                with "Hla Hep Hdisj"). iExact "Harm". }
+                wl wdu wdt gl cl rl pl fz cn Hlok Hrt Hdir Hwl0 Hpar Hclm Hfrz
+                with "Hla Hep Hdisj Hcnt Hfdisj"). iExact "Harm". }
     iModIntro. iFrame "Hdn Hfrag". iPureIntro. exact Hty.
   Qed.
 
